Don't emit Coq modules for Go interfaces;
updated gold

internal/coq/coq.go
@@ -155,13 +155,10 @@ type InterfaceDecl struct {
 	Comment string
 }
 
-// FIXME: update these to not use modules
 func (d InterfaceDecl) CoqDecl() string {
 	var pp buffer
 	pp.AddComment(d.Comment)
-	pp.Add("Module %s.", d.Name)
-	pp.Indent(2)
-	pp.AddLine("Definition S := struct.decl [")
+	pp.Add("Definition %s := struct.decl [", d.Name)
 	pp.Indent(2)
 	for i, fd := range d.Methods {
 		sep := ";"
@@ -172,17 +169,13 @@ func (d InterfaceDecl) CoqDecl() string {
 	}
 	pp.Indent(-2)
 	pp.AddLine("].")
-	pp.Indent(-2)
-	pp.Add("End %s.", d.Name)
 	return pp.Build()
 }
 
 func (d InterfaceDecl) Coq() string {
 	var pp buffer
 	pp.AddComment(d.Comment)
-	pp.Add("Module %s.", d.Name)
-	pp.Indent(2)
-	pp.AddLine("Definition S := struct.decl [")
+	pp.Add("Definition %s := struct.decl [", d.Name)
 	pp.Indent(2)
 	for i, fd := range d.Methods {
 		sep := ";"
@@ -193,8 +186,6 @@ func (d InterfaceDecl) Coq() string {
 	}
 	pp.Indent(-2)
 	pp.AddLine("].")
-	pp.Indent(-2)
-	pp.Add("End %s.", d.Name)
 	return pp.Build()
 }
 
@@ -212,9 +203,9 @@ func (d StructToInterface) Coq() string {
 		pp.Add("rec: \"%s_to_%s\" \"t\" :=", d.Struct, d.Interface)
 		pp.Indent(2)
 		if len(d.Methods) == 1 {
-			pp.Add("struct.mk %s.S [\"%s\" ::= %s__%s \"t\"].", d.Interface, d.Methods[0], d.Struct, d.Methods[0])
+			pp.Add("struct.mk %s [\"%s\" ::= %s__%s \"t\"].", d.Interface, d.Methods[0], d.Struct, d.Methods[0])
 		} else {
-			pp.Add("struct.mk %s.S [", d.Interface)
+			pp.Add("struct.mk %s [", d.Interface)
 			pp.Indent(2)
 			for i, method := range d.Methods {
 				if i == len(d.Methods)-1 {
@@ -1103,7 +1094,7 @@ func StructMethod(structName string, methodName string) string {
 }
 
 func InterfaceMethod(interfaceName string, methodName string) string {
-	return fmt.Sprintf("struct.get %s.S \"%s\"", interfaceName, methodName)
+	return fmt.Sprintf("struct.get %s \"%s\"", interfaceName, methodName)
 }
 
 // TODO: note that the second two lines should be customized depending on the
