internal/examples/append_log/append_log.gold.v
@@ -10,28 +10,26 @@ From Goose Require github_com.tchajed.marshal.
    appends, which are implemented by atomically updating an on-disk header with
    the number of valid blocks in the log. *)
 
-Module Log.
-  Definition S := struct.decl [
-    "m" :: lockRefT;
-    "sz" :: uint64T;
-    "diskSz" :: uint64T
-  ].
-End Log.
+Definition Log := struct.decl [
+  "m" :: lockRefT;
+  "sz" :: uint64T;
+  "diskSz" :: uint64T
+].
 
 Definition Log__mkHdr: val :=
   rec: "Log__mkHdr" "log" :=
     let: "enc" := marshal.NewEnc disk.BlockSize in
-    marshal.Enc__PutInt "enc" (struct.loadF Log.S "sz" "log");;
-    marshal.Enc__PutInt "enc" (struct.loadF Log.S "diskSz" "log");;
+    marshal.Enc__PutInt "enc" (struct.loadF Log "sz" "log");;
+    marshal.Enc__PutInt "enc" (struct.loadF Log "diskSz" "log");;
     marshal.Enc__Finish "enc".
-Theorem Log__mkHdr_t: ⊢ Log__mkHdr : (struct.ptrT Log.S -> disk.blockT).
+Theorem Log__mkHdr_t: ⊢ Log__mkHdr : (struct.ptrT Log -> disk.blockT).
 Proof. typecheck. Qed.
 Hint Resolve Log__mkHdr_t : types.
 
 Definition Log__writeHdr: val :=
   rec: "Log__writeHdr" "log" :=
     disk.Write #0 (Log__mkHdr "log").
-Theorem Log__writeHdr_t: ⊢ Log__writeHdr : (struct.ptrT Log.S -> unitT).
+Theorem Log__writeHdr_t: ⊢ Log__writeHdr : (struct.ptrT Log -> unitT).
 Proof. typecheck. Qed.
 Hint Resolve Log__writeHdr_t : types.
 
@@ -39,20 +37,20 @@ Definition Init: val :=
   rec: "Init" "diskSz" :=
     (if: "diskSz" < #1
     then
-      (struct.new Log.S [
+      (struct.new Log [
          "m" ::= lock.new #();
          "sz" ::= #0;
          "diskSz" ::= #0
        ], #false)
     else
-      let: "log" := struct.new Log.S [
+      let: "log" := struct.new Log [
         "m" ::= lock.new #();
         "sz" ::= #0;
         "diskSz" ::= "diskSz"
       ] in
       Log__writeHdr "log";;
       ("log", #true)).
-Theorem Init_t: ⊢ Init : (uint64T -> (struct.ptrT Log.S * boolT)).
+Theorem Init_t: ⊢ Init : (uint64T -> (struct.ptrT Log * boolT)).
 Proof. typecheck. Qed.
 Hint Resolve Init_t : types.
 
@@ -62,32 +60,32 @@ Definition Open: val :=
     let: "dec" := marshal.NewDec "hdr" in
     let: "sz" := marshal.Dec__GetInt "dec" in
     let: "diskSz" := marshal.Dec__GetInt "dec" in
-    struct.new Log.S [
+    struct.new Log [
       "m" ::= lock.new #();
       "sz" ::= "sz";
       "diskSz" ::= "diskSz"
     ].
-Theorem Open_t: ⊢ Open : (unitT -> struct.ptrT Log.S).
+Theorem Open_t: ⊢ Open : (unitT -> struct.ptrT Log).
 Proof. typecheck. Qed.
 Hint Resolve Open_t : types.
 
 Definition Log__get: val :=
   rec: "Log__get" "log" "i" :=
-    let: "sz" := struct.loadF Log.S "sz" "log" in
+    let: "sz" := struct.loadF Log "sz" "log" in
     (if: "i" < "sz"
     then (disk.Read (#1 + "i"), #true)
     else (slice.nil, #false)).
-Theorem Log__get_t: ⊢ Log__get : (struct.ptrT Log.S -> uint64T -> (disk.blockT * boolT)).
+Theorem Log__get_t: ⊢ Log__get : (struct.ptrT Log -> uint64T -> (disk.blockT * boolT)).
 Proof. typecheck. Qed.
 Hint Resolve Log__get_t : types.
 
 Definition Log__Get: val :=
   rec: "Log__Get" "log" "i" :=
-    lock.acquire (struct.loadF Log.S "m" "log");;
+    lock.acquire (struct.loadF Log "m" "log");;
     let: ("v", "b") := Log__get "log" "i" in
-    lock.release (struct.loadF Log.S "m" "log");;
+    lock.release (struct.loadF Log "m" "log");;
     ("v", "b").
-Theorem Log__Get_t: ⊢ Log__Get : (struct.ptrT Log.S -> uint64T -> (disk.blockT * boolT)).
+Theorem Log__Get_t: ⊢ Log__Get : (struct.ptrT Log -> uint64T -> (disk.blockT * boolT)).
 Proof. typecheck. Qed.
 Hint Resolve Log__Get_t : types.
 
@@ -101,41 +99,41 @@ Hint Resolve writeAll_t : types.
 
 Definition Log__append: val :=
   rec: "Log__append" "log" "bks" :=
-    let: "sz" := struct.loadF Log.S "sz" "log" in
-    (if: slice.len "bks" ≥ struct.loadF Log.S "diskSz" "log" - #1 - "sz"
+    let: "sz" := struct.loadF Log "sz" "log" in
+    (if: slice.len "bks" ≥ struct.loadF Log "diskSz" "log" - #1 - "sz"
     then #false
     else
       writeAll "bks" (#1 + "sz");;
-      struct.storeF Log.S "sz" "log" (struct.loadF Log.S "sz" "log" + slice.len "bks");;
+      struct.storeF Log "sz" "log" (struct.loadF Log "sz" "log" + slice.len "bks");;
       Log__writeHdr "log";;
       #true).
-Theorem Log__append_t: ⊢ Log__append : (struct.ptrT Log.S -> slice.T disk.blockT -> boolT).
+Theorem Log__append_t: ⊢ Log__append : (struct.ptrT Log -> slice.T disk.blockT -> boolT).
 Proof. typecheck. Qed.
 Hint Resolve Log__append_t : types.
 
 Definition Log__Append: val :=
   rec: "Log__Append" "log" "bks" :=
-    lock.acquire (struct.loadF Log.S "m" "log");;
+    lock.acquire (struct.loadF Log "m" "log");;
     let: "b" := Log__append "log" "bks" in
-    lock.release (struct.loadF Log.S "m" "log");;
+    lock.release (struct.loadF Log "m" "log");;
     "b".
-Theorem Log__Append_t: ⊢ Log__Append : (struct.ptrT Log.S -> slice.T disk.blockT -> boolT).
+Theorem Log__Append_t: ⊢ Log__Append : (struct.ptrT Log -> slice.T disk.blockT -> boolT).
 Proof. typecheck. Qed.
 Hint Resolve Log__Append_t : types.
 
 Definition Log__reset: val :=
   rec: "Log__reset" "log" :=
-    struct.storeF Log.S "sz" "log" #0;;
+    struct.storeF Log "sz" "log" #0;;
     Log__writeHdr "log".
-Theorem Log__reset_t: ⊢ Log__reset : (struct.ptrT Log.S -> unitT).
+Theorem Log__reset_t: ⊢ Log__reset : (struct.ptrT Log -> unitT).
 Proof. typecheck. Qed.
 Hint Resolve Log__reset_t : types.
 
 Definition Log__Reset: val :=
   rec: "Log__Reset" "log" :=
-    lock.acquire (struct.loadF Log.S "m" "log");;
+    lock.acquire (struct.loadF Log "m" "log");;
     Log__reset "log";;
-    lock.release (struct.loadF Log.S "m" "log").
-Theorem Log__Reset_t: ⊢ Log__Reset : (struct.ptrT Log.S -> unitT).
+    lock.release (struct.loadF Log "m" "log").
+Theorem Log__Reset_t: ⊢ Log__Reset : (struct.ptrT Log -> unitT).
 Proof. typecheck. Qed.
 Hint Resolve Log__Reset_t : types.
